
## Projections

What is a projection?

In a plane, with a coordinate system R=(O,i,j), we can give two distinct lines d and g, that pass through O.

To project a point M onto d would be to move M along a line // to g, until it reaches d.

If M is already on d, then M'=M.
All points on g have their M'=O.

If we introduce coordinates to this:

M = (x, y)
M' = (x', y')

We also introduce a point ($\lambda, \mu$) and a point ($-\sigma, \rho$). We can also define g to be $\rho x+ \sigma y$.

We also define that $\vec{u}=\vec{OM}$ and $\vec{u}'=\vec{OM'}$, $\vec{u}$ being also $\binom{x}{y}$ and $\vec{u'}=\binom{x'}{y'}$.

A proposition we have, which is also really the analytical definition of projection on d parallel to g has the following analytical expression:

$$
\begin{split}
p:\begin{bmatrix}x'\\y'\end{bmatrix}=P\begin{bmatrix}x\\y\end{bmatrix}\\
P= \frac{1}{\lambda\rho+\mu\sigma}\begin{bmatrix}\lambda\\ \mu\end{bmatrix}\begin{bmatrix}\rho &\sigma \end{bmatrix}=\begin{bmatrix} \frac{\lambda\rho}{\lambda\rho+\mu\sigma}& \frac{\lambda\sigma}{\lambda\rho+\mu\sigma}\\ \frac{\mu\rho}{\lambda\rho+\mu\sigma}& \frac{\mu\sigma}{\lambda\rho+\mu\sigma}\end{bmatrix}
\end{split}
$$

It's worth noting that $\frac{1}{\lambda\rho+\mu\sigma}$ insures normalization, so that $tr (P)= 1$.
$\begin{bmatrix}\lambda\\ \mu\end{bmatrix}$ is the director vector of d, and $\begin{bmatrix}\rho &\sigma \end{bmatrix}$ is the equation of g.

The proof is as follows:

In the base $B=(\lambda, \mu),(-\sigma, \rho)$, we have $(x, y)=t_{1}(\lambda, \mu)+t_{2}(-\sigma, \rho)$.

This means:

$$
\begin{bmatrix}t_{1}\\ t_{2}\end{bmatrix}=\begin{bmatrix}\lambda & -\sigma \\ \mu & \rho\end{bmatrix}^{-1}\begin{bmatrix}x \\ y\end{bmatrix} = \frac{1}{\lambda\rho+\mu\sigma}\begin{bmatrix} \rho & \sigma \\ -\mu & \lambda \end{bmatrix}\begin{bmatrix}x \\ y\end{bmatrix}
$$

Fascinating. This also means:

$$
\begin{bmatrix}x'\\ y'\end{bmatrix}=t_{1}\begin{bmatrix}\lambda\\ \mu\end{bmatrix}= \frac{\rho x+ \sigma y}{\lambda \rho+\mu\sigma}\begin{bmatrix}\lambda\\ \mu\end{bmatrix}=\frac{1}{\lambda\rho+\mu\sigma}\begin{bmatrix} \rho & \sigma \\ -\mu & \lambda \end{bmatrix}\begin{bmatrix}x \\ y\end{bmatrix}
$$

Matrices that appear in this way are called **projection matrices**.

Proposition: these are exactly the matrices $P=\begin{bmatrix}\alpha&\beta\\\gamma & \delta\end{bmatrix}$, with: $\begin{cases}tr(P)=1\\ \det(P)=0\end{cases}$

the proof $\implies$ is clear, by definition. However the $\impliedby$ is more complex.

Let's notice that $\det(P)=0$, means that automagically, $rg(P)\le1$, and therefore:

$$
P=\begin{bmatrix}\lambda\\\mu\end{bmatrix}\begin{bmatrix}\rho& \sigma\end{bmatrix}=\begin{bmatrix}\lambda\rho&\lambda\sigma\\ \mu\rho& \mu\sigma\end{bmatrix}=\frac{1}{\lambda\rho+\mu\sigma}\begin{bmatrix}\lambda\\ \mu\end{bmatrix}\begin{bmatrix}\rho& \sigma\end{bmatrix}
$$

Which proves it. 

### Example 1

The projection p on $d: 3x+y=0$ in parallel to $g: y=x$ has the following matrix:

$$
P=\begin{bmatrix}1\\-3\end{bmatrix}\begin{bmatrix}1&-1\end{bmatrix}= \frac{1}{4}\begin{bmatrix}1 & -1\\-3 & 3\end{bmatrix}
$$

> [!note]+
>as a reminder, the director vector of a line (d here), is given for $ax+by=c$ by $(b, -a)$, while the normal is $(a, b)$


Which means the formula here is:

$$
p: \begin{cases}x'= \frac{1}{4}x- \frac{1}{4}y\\ y'=- \frac{3}{4}x+ \frac{3}{4}y\end{cases}
$$

### Example 2

Give the nature and characteristics of the following transformation:

$$
\begin{cases}x'= \frac{1}{7}x+ \frac{2}{7}y]\\ y'= \frac{3}{7}x+ \frac{6}{7}y\end{cases}\iff\begin{bmatrix}x'\\ y'\end{bmatrix}=\begin{bmatrix} \frac{1}{7}& \frac{2}{7}\\ \frac{3}{7} & \frac{6}{7}\end{bmatrix}\begin{bmatrix}x\\ y\end{bmatrix}
$$

as $tr(P)=1$, and $\det(P)=0$, it's a projection[^1] p (whose axes pass through the origin). Let's find d and g !

We have a couple of methods:

#### Method 1

$$
P= \frac{1}{7}\begin{bmatrix}1\\3\end{bmatrix}\begin{bmatrix}1&2\end{bmatrix}\implies\begin{cases}d:3x-y=0\\ g:x+2y=0\end{cases}
$$


#### Method 2

$$
d:\begin{cases}x'=x\\ y'=y\end{cases}\implies\begin{cases} \frac{1}{7}x+ \frac{2}{7}y=x\\ \frac{3}{7}x+ \frac{6}{7}y=y\end{cases}\implies y=3x
$$

and 

$$
g:\begin{cases}x'=0\\ y'=0\end{cases}\implies\begin{cases} \frac{1}{7}x+ \frac{2}{7}y=0\\ \frac{3}{7}x+ \frac{6}{7}y=0\end{cases}\implies x+2y=0
$$

Which is the same answers.

#### Method 3

This is the point-image couple method.

If A(7, 0), then A'(1, 3). We thus have $d=OA'$, $y = 3x$, and AA' is (-6, 3), which gives us $g:x+2y=0$


#### Summary

By either decomposing the matrix, solving it in a general case, or solving it in a specific case, we'll find the equations of both lines.

Method 1 is fastest when the matrix is obvious, 2 always works, 3 is faster than 2, but a point needs to be obvious.

## Symmetries

First of all, same notation as for the first part, meaning we have d, and g, and M and M'.

However this time M' is in a bit of a different spot.

It's basically found in two steps: first, we project M onto d, and then we keep going in the direction of g.

If we add the coordinates back in: $M'(x',y')=S(M)$.

If M'=M, it means M is part of d.

Because of all of this, P(M) is the middle of MM', that is to say $\frac{1}{2}(\begin{bmatrix}x'\\ y'\end{bmatrix}+\begin{bmatrix}x\\ y\end{bmatrix})=P\begin{bmatrix}x\\ y\end{bmatrix}$.

All that to say: $\begin{bmatrix}x'\\ y'\end{bmatrix}=2P\begin{bmatrix}x\\ y\end{bmatrix}-\begin{bmatrix}x\\ y\end{bmatrix}$.

Proposition: symmetry in relation to d parallel to g has as expression:

$$
s:\begin{bmatrix}x' \\ y'\end{bmatrix}=S\begin{bmatrix}x\\ y\end{bmatrix}\text{ where } S=2P-I_{2}
$$

P being what we saw in the first part.

This means all S matrices have some fun properties, notably that  their trace is 0, and their determinant is of -1.

In math terms:

$$
S=\begin{bmatrix}\alpha&\beta\\\gamma&\delta\end{bmatrix}\iff\begin{cases}
tr(S)=0\implies \alpha+\delta=0\\ \\
\det(S)=-1\implies \alpha\delta-\beta\gamma=-1
\end{cases}
$$

The proof is 

$$
P= \frac{1}{2}(I_{2} +S)= \frac{1}{2}\begin{bmatrix}\alpha+1 & \beta \\ \gamma& \delta+1\end{bmatrix}
$$

We thus have:

$$
\begin{cases} tr(S)=0 \\ \det(S)=-1 \end{cases} \iff \begin{cases}tr(P)= \frac{1}{2}(\alpha+\delta+2)=1\iff \alpha+\delta=0 \\ \det(P)= \frac{1}{4}(1+\alpha+\delta+\alpha\delta-\beta\gamma=0\end{cases}
$$

We also say that P is the projection matrix associated with S.

### Example 1

The symmetry with regards to $d: 3x+y=0$ parallel to $g: y=x$ has as matrix $S\in M_{2}(\mathbb{R})$ so that:

$$
\frac{1}{2}(I_{2}+S)=P\iff S=2P-I_{2}=??
$$

We know that P here is $\begin{bmatrix}1&-1\\-3&3\end{bmatrix}$.

This means:

$$
\frac{1}{2}\begin{bmatrix}-1&-1\\-3&1\end{bmatrix}
$$

### Example 2

Give the nature and the characteristic elements of the transformation:

$$
\begin{cases} x'=2x+3y\\y'=-x-2y \end{cases}\iff \begin{bmatrix}x'\\y'\end{bmatrix}=\begin{bmatrix}2&3\\-1&-2\end{bmatrix}\begin{bmatrix}x\\y\end{bmatrix}
$$

We can find that $tr$ is 0 and $\det$ is -1, which means it is a symmetry, whose axes d and g go through the origin.
Let's find them.

#### Method 1

Using method 1, the associated projection:

$$
P= \frac{1}{2}(I_{2}+S)=\frac{1}{2}\begin{bmatrix}3&3\\-1&-1\end{bmatrix}= \frac{1}{2}\begin{bmatrix}3\\-1\end{bmatrix}\begin{bmatrix}1&1\end{bmatrix}
$$

This means d has $\begin{bmatrix}3\\-1\end{bmatrix}$ as director vector, meaning it's formula is $x+3y$, and g is has $\begin{bmatrix}1&1\end{bmatrix}$, meaning it's defined as $f:x+y=0$.


#### Method 2

Let's find the fixed points:

$$
M'=M\implies d:\begin{cases}x'=x\\y'=y\end{cases}\iff\begin{cases}2x+3y=x\\ -x-2y=y\end{cases}\iff x+3y=0
$$

As for g:

$$
M'=-M\implies g: \begin{cases}x'=-x\\ y'=-y\end{cases}\iff\begin{cases}2x+3y=-x\\ -x-2y=-y\end{cases}\iff g:x+y=0
$$
### Method 3

Let's use a random point (point-image couple)

if A(1, 0), then A' (2, -1).

We can easily find the middle: ($\frac{3}{2}, - \frac{1}{2}$).

From there, we can proceed to find g:

$$
x+3y=0 \implies g: x+y=0
$$



[[7. Rotations|Previous]]

[^1]:also hinted at by the name of the chapter
