
## How to turn a vector by an angle

Say we have a $\vec{v}=\binom{x}{y}$.

If we turn it by an angle $\beta$ in the positive direction, we obtain a vector $\vec{v}$ whose coordinates are: $\vec{v}=\begin{pmatrix} x\cos(\beta)-y\sin{\beta} \\ x\sin(\beta)+y\cos(\beta) \end{pmatrix}$.

To prove this, is quite a geometric task, if you draw what it entails on a circle it becomes quite clear. Unfortunately, drawings is not one of the things I've figured out how to do in this notes system. If by say November I haven't done that, someone remind me.

Anyhow, in math terms, if we turn vectors $\vec{i}$ and $\vec{j}$ (the director vectors of the plane), as well as $\vec{v}$ by $\beta$, that's the same as if the entire plane rotated by $\beta$, but nothing changed.

Luckily, we can also reference all that in terms of the original plane, so we can determine the new values of $\vec{i}$ and $\vec{j}$.

$$
\vec{i}=\binom{\cos\beta}{\sin\beta}\text{ and }\vec{j}=\binom{-\sin\beta}{\cos\beta} 
$$

From there, we know that compared to the new i and j, v hasn't changed, therefore:

$$
\vec{v}=x\binom{\cos\beta}{\sin\beta}+y\binom{-\sin\beta}{\cos\beta}=\vec{v}=\begin{pmatrix} x\cos(\beta)-y\sin{\beta} \\ x\sin(\beta)+y\cos(\beta) \end{pmatrix}
$$

## Sum and difference identities

$\forall\alpha\beta\in\mathbb{R}$

$cos(A-B)=cos(A)\times cos(B) + sin(A)\times sin(B)$
$cos(A+B)=cos(A)\times cos(B) - sin(A)\times sin(B)$
$sin(A+B)=sin(A)\times cos(B) + cos(A)\times sin(B)$
$sin(A-B)=sin(A)\times cos(B) - cos(A)\times sin(B)$

the proof is as follows:

We choose $\vec{v}=\binom{\cos{\alpha}}{\sin{\alpha}}$

If we turn it by an angle $\beta$, we get that $\vec{v}=\binom{\cos(\alpha+\beta)}{\sin(\alpha+\beta)}$

From before, we also know it's $\begin{pmatrix} x\cos(\beta)-y\sin{\beta} \\ x\sin(\beta)+y\cos(\beta) \end{pmatrix}$.

This allows us to deduce that:

$\cos(\alpha+\beta)=\cos(\alpha)\cos(\beta)-\sin(\alpha)\sin(\beta)$
and
$\sin(\alpha+\beta)=\cos(\alpha)\sin(\beta)+\sin(\alpha)\cos(\beta)$

\- is also trivial to deduce from all that.

As for tan and cot:

$tan(A+B)=\cfrac{tan(A)+tan(B)}{1-tan(A)\times tan(B)}$

$cot(A+B)=\cfrac{cot(B)cot(A)-1}{cot(B)+cot(A)}$

How do we get that:

$\tan(\alpha+\beta)= \frac{\sin(\alpha+\beta)}{\cos(\alpha+\beta)}$

That turns into:

$\tan(\alpha+\beta)= \cfrac{\cos(\alpha)\sin(\beta)+\sin(\alpha)\cos(\beta)}{\cos(\alpha+\beta)=\cos(\alpha)\cos(\beta)-\sin(\alpha)\sin(\beta)}$

Which can be turned not without effort, but with enough simplification and division, into

$$
\tan(\alpha+\beta)=\frac{\frac{\sin(\alpha)\cos(\beta)+\sin(\beta)\cos(\alpha)}{\cos(\alpha)\cos(\beta)}}{\frac{\cos(\alpha)\cos(\beta)-\sin(\alpha)\sin(\beta)}{\cos(\alpha)\cos(\beta)}}
$$

Which is equivalent to $tan(A+B)=\cfrac{tan(A)+tan(B)}{1-tan(A)\times tan(B)}$

cot is essentially the same.

## Bisection formulas

We have $cos(\alpha)=1-2\sin^{2}( \frac{\alpha}{2})=2\sin^{2}( \frac{\alpha}{2})-1$

$\forall \alpha\in\mathbb{R}$
$\cos^{2}( \frac{\alpha}{2})= \frac{1+\cos(\alpha)}{2}$
$\sin^{2}(\frac{\alpha}{2})= \frac{1-\cos(\alpha)}{2}$

We know if $\frac{\alpha}{2}\in D_{tan}$ then $tan^{2}(\frac{\alpha}{2})=\frac{1-cos\alpha}{1+cos\alpha}$
and if $\frac{\alpha}{2}\in D_{cot}$ then $tan^{2}( \frac{\alpha}{2})=1+\frac{cos\alpha}{1-cos(\alpha)}$
so depending on the value its in a part of quadrant 1 to 4, allowing us to find the sign.

This feels like overengineering. 

## transformation sum-product

Say $\forall \alpha,\beta\in \mathbb{R}$

$\sin(\alpha)+\sin(\beta)=2\sin( \frac{\alpha+\beta}{2})\cos( \frac{\alpha-\beta}{2})$
$\sin(\alpha)-\sin(\beta)=2\cos( \frac{\alpha+\beta}{2})\sin( \frac{\alpha-\beta}{2})$

$\cos(\alpha)+\cos(\beta)=2\cos( \frac{\alpha+\beta}{2})\sin( \frac{\alpha-\beta}{2})$
$\cos(\alpha)-\cos(\beta)=2\sin( \frac{\alpha+\beta}{2})\cos( \frac{\alpha-\beta}{2})$

The proof is:

$\forall \gamma,\delta\in\mathbb{R}$

1) $sin(\gamma+\delta)=sin(\gamma)cos(\delta)+sin(\delta)cos(\gamma)$
2) $sin(\gamma-\delta)=sin(\gamma)cos(\delta)-sin(\delta)cos(\gamma)$

By adding 1 and 2:

3) $\sin(\gamma+\delta)+sin(\gamma-\delta)=2sin(\gamma)cos(\delta)$

By subtracting 2 to 1, we get

4) $sin(\gamma+\delta)-sin(\gamma-\delta)=2sin(\delta)cos(\gamma)$

By setting:

$\begin{cases}\alpha=\gamma+\delta \\ \beta=\gamma-\delta\end{cases}\iff\begin{cases} \gamma= \frac{\alpha+\beta}{2}\\ \delta= \frac{\alpha-\beta}{2}\end{cases}$

And by replacing that, we get

$\sin(\alpha)+\sin(\beta)=2\sin( \frac{\alpha+\beta}{2})\cos( \frac{\alpha-\beta}{2})$
$\sin(\alpha)-\sin(\beta)=2\cos( \frac{\alpha+\beta}{2})\sin( \frac{\alpha-\beta}{2})$

which is what we were trying to prove.

cos is proven in the same way.
## Examples

### Ex 1

Solve $cos(x)+cos(\frac{\pi}{3}-x)=sin(\frac{\pi}{3})$

$$
\begin{equation}
\begin{split}
cos(x)+cos(\frac{\pi}{3}-x)=sin(\frac{\pi}{3})\\
\iff 2cos(\frac{\pi}{6})cos(\frac{2x- \frac{\pi}{3}}{2})=sin(\frac{\pi}{3})\\
\iff 2\frac{\sqrt{3}}{2}cos(x- \frac{\pi}{6})=\frac{\sqrt{3}}{3}\\
\iff cos(x- \frac{\pi}{6})=\frac{1}{2} \\
\iff x- \frac{\pi}{6}=
    \begin{cases}
    \frac{\pi}{3}+2\pi k, k\in\mathbb{Z}\\\\
    - \frac{\pi}{3}+2\pi k, k\in\mathbb{Z}
    \end{cases}
\\\\
\iff x = 
    \begin{cases}
    \frac{\pi}{2}+2\pi k, k\in\mathbb{Z}\\\\ \\
    - \frac{\pi}{2}+2\pi k, k\in\mathbb{Z}
    \end{cases}
\end{split}
\end{equation}
$$
### Ex 2

Calculate $\tan(\frac{\pi}{12})$

Well, $\frac{\pi}{12}= \frac{3\pi}{12}- \frac{2\pi}{12}=\frac{\pi}{4}- \frac{\pi}{6}$

So, we need to solve $\tan(\frac{\pi}{4}- \frac{\pi}{6})$

$$
\iff \frac{\tan(\frac{\pi}{4})-\tan(\frac{\pi}{6})}{1+\tan(\frac{\pi}{4})\tan(\frac{\pi}{6})}
$$

$$
\iff  \frac{1- \frac{\sqrt{3}}{3}}{1+ \frac{\sqrt{3}}{3}}
$$



### Ex 3 - with inequalities

Solve $\cos^{2}(\frac{3}{2}x)- \frac{1}{2}\ge \frac{\sqrt{3}}{4}$, $x\in[-2\pi, -\pi]$

First, we solve this regularly, to get to:

$- \frac{\pi}{18}+ \frac{2\pi}{3}k\le x \le \frac{\frac{pi}{18}+2\pi}{3}k, k\in\mathbb{Z}$

Then, we know that:

$x\in[-2\pi;\pi]$,  $x\in\mathrm{I}\bigcup\mathrm{II}$

and as it's in the $-2\pi$ range, we need to subtract $2pi=(\frac{36\pi}{18}$) to the intervals we got before, to get:

$S=[-2\pi; \frac{-33\pi}{18}]\bigcup[ \frac{-25\pi}{18}; \frac{-23\pi}{18}]$


[[3. Elementary Trig Equations|Previous]]
[[5. Linear equations|Next]]
