
To make functions have a reciprocal function is not trivial, particularly in the case of functions like sine and cosine.

To make any function bijective, you need to restrain it's input and output set.
The output set is simple: 
we turn $f:D_{f}\to \mathbb{R}$
into $f:D_{f}\to Im(f)$
this gives us a surjective function

We then need to turn a function injective, so that we don't map twice to the same value
For example $f:\mathbb{R}\to\mathbb{R}, x\to x^2$  is not injective, but $f:\mathbb{R}_{+}\to\mathbb{R}_{+},x\to x^{2}$ is.

## Sine

Sine can be represented as $\sin:\mathbb{R}\to[-1,1]$

it is surjective, however it is not injective.

We thus need to reduce it's input set, that much is obvious, but to what?
We could chose $[- \frac{\pi}{2}, \frac{\pi}{2}]$.

Technically ll intervals of the form $[-\frac{\pi}{2}+k \pi, \frac{\pi}{2}+k \pi]$ where $k\in\mathbb{Z}$.
We choose by convention $[- \frac{\pi}{2}, \frac{\pi}{2}]$

We now have the bijective function $\sin [-\frac{pi}{2},\frac{pi}{2}]\to[-1,1]$

It's reciprocal function, which we call arcsine, and write either $\arcsin$ or $\sin^{-1}$

$\arcsin:[-1;1]\to[- \frac{\pi}{2}, \frac{\pi}{2}], x\to y|\sin(y)=x$

arc-sine is thus the only angle between $- \frac{\pi}{2}$ and $\frac{\pi}{2}$, the sine of which is x.

This also means:

$\sin(\arcsin(x))=x$
but $\arcsin(\sin(x))\ne x$ most of the time
$\arcsin(\sin(x))= x\iff x\in[- \frac{\pi}{2}, \frac{\pi}{2}]$
$\arcsin(-x)=-\arcsin(x)$

$-\arcsin(x)\in[- \frac{\pi}{2}, \frac{\pi}{2}]$

$\sin(-\arcsin(x))=-\sin(\arcsin(x))=-x$


Arcsine's only real power is allowing us to solve exercises without going through special values ($\frac{\pi}{2},\frac{\pi}{3}$...)
We simply write:

$\begin{cases}\arcsin(a)+2\pi k\\\pi-\arcsin(a)+2\pi k\end{cases}$

### Example

Solve $\sin(x)=-\frac{3}{4}$ on $x\in[\pi, 2\pi]$

$\begin{cases}\arcsin(- \frac{3}{4})+2\pi k\\ \arcsin{\pi-\arcsin(\frac{-3}{4}+2\pi k)} \end{cases}$

$\arcsin(\frac{-3}{4})+2\pi\in [\frac{3\pi}{2},2\pi]$
=> $\pi-\arcsin(\frac{-3}{4})\in[\pi,\frac{3\pi}{2}]$

S = $\arcsin{\frac{-3}{4}}+2\pi, \pi-\arcsin(\frac{-3\pi}{4})$



### Trigonometric function in arcsines

1. $\sin(\arcsin(x))=x, \forall x\in[-1,1]$
2. $\cos(\arcsin(x))=+\sqrt{1-\sin^{2}(\arcsin(x))}=\sqrt{1-x^{2}}$
3. $\tan(\arcsin(x))=\frac{\sin(\arcsin)}{\cos(\arcsin)}=\frac{x}{\sqrt{1+x^{2}}}$


## Cosine

We restrain cosine in $[0, \pi]$, that way we make it bijective, in much the same way as we did with sine. This one is also defined by convention.

So, we get $\cos:[0,\pi]\to[-1,1]$
It's reciprocal function will be $\arccos:[-1,1]\to[0,\pi]$

Some of it's properties include:

$\cos(\arccos(x))=x,\forall x\in[-1,1]$
$\arccos(\cos(x))\ne x$ typically,
if $\arccos(\cos(x))=x\iff x\in[0,\pi]$

$\arccos(-x)=\pi-\arccos(x)\forall x\in[-1,1]$

Much like with arcsine, we can use arccos to solve equations:

the solution for $\cos(x)=a,a\in[-1,1]$ is then
$\begin{cases}\arccos(x)+2\pi k \\ -\arccos(x)+2\pi k\end{cases}$

### Example

Solve $\cos(x)\le \frac{-3}{4}$ for $x\in[\frac{-3\pi}{2},-\pi]$

We can find $\frac{-\sqrt{3}}{2}\lt \frac{-3}{4}\lt \frac{-1}{2}\iff \cos(\frac{5\pi}{2})\lt \frac{-3}{4}\lt \cos(\frac{2pi}{3})$

Which means

$\frac{2\pi}{3}\lt \arccos(\frac{-3}{4})\lt \frac{5\pi}{6}$

Using this we can roughly place it on a trig circle. We then need to put there the symmetry as well, so we get the solutions for if it was =, however we have lesser or equal and we're limited to an interval, so we need to write the following:

$\cos(x)\le \frac{-3}{4}\iff -\arccos(\frac{-3}{4})+2\pi k\le x\le2\pi-\arccos(\frac{-3}{4})+2\pi k$

In $[\frac{-3\pi}{2},-\pi]$ it's thus $S=[\arccos(\frac{-3}{4})-2\pi, -\pi]$

### Trig functions in arccosine

$\cos(\arccos(x))=x \forall x \in[-1,1]$
$\sin(\arccos(x))=\sqrt{1-\cos^{2}(\arccos(x))}=\sqrt(1-x^{2})$
$\tan(\arccos(x))=\frac{\sqrt{1-x^{2}}}{x}$


## Tangent

The definition of the tangent is, again by convention, $] \frac{-pi}{2}, \frac{\pi}{2}[$

$\tan:] \frac{-pi}{2}, \frac{\pi}{2}[\to\mathbb{R}$

and thus arctan is $\arctan: \mathbb{R}\to ]\frac{-pi}{2}, \frac{\pi}{2}[$


It's properties are:

$\tan(\arctan(x))=x\forall x\in\mathbb{R}$
$\arctan(\tan(x))=x\iff x\in] \frac{-pi}{2}, \frac{\pi}{2}[$
$\arctan(-x)=-\arctan(x)$
$\tan(x)=a, a\in\mathbb{R}$ has a solution of $x=\arctan(a)+k\pi$

## Example
$\tan(x)\le 5,x\in\mathbb{R}$

$\frac{-\pi}{2}+k \pi\lt x \le \arctan(5)+ k \pi$


## Trig functions in arctan

$\tan(\arctan(x))=x$
$\forall\alpha\in] \frac{-\pi}{2}, \frac{\pi}{2}[$

$\sin(x)=\tan(\alpha)\cos(\alpha)=\tan(\alpha)\sqrt{1-\sin^{2}(\alpha)}$
$\iff \sin^{2}(\alpha)=\tan^{2}(\alpha)(1-\sin^{2}(\alpha))$
$\iff\sin^{2}(\alpha)(1+\tan^{2}(\alpha))=\tan^{2}\alpha$
$\iff\sin^{2}(\alpha)=\frac{\tan^{2}(\alpha)}{1+\tan^{2}(\alpha)}\iff\sin(\alpha)= \frac{\tan(\alpha)}{\sqrt{1+\tan^{2}(\alpha)}}$

Which means $\sin(\arctan(x))=\frac{\tan(\arctan(x))}{\sqrt{1-\tan^{2}(\arctan(x))}}= \frac{x}{\sqrt{1+x^{2}}}$

which allows us to say:
$\cos(\arctan(x))=\frac{1}{\sqrt{1+x^{2}}}$

### Example 2

Find $\arctan(2)+\arctan(3)$

If we define $\alpha=\arctan(2)$ and $\beta=\arctan(3)$...

$\tan(\alpha+\beta)= \frac{\tan(\alpha)+\tan(\beta)}{1-\tan(\alpha)\tan(\beta)}$
which as we know is $\frac{2+3}{1-2*3}=-1$

so that $\tan(\alpha+\beta)=-1$, we need $\alpha+\beta=\arctan(-1)+k\pi$

which we know to be $\frac{-\pi}{4}+k\pi$
As we know, $\arctan(2)\in[0,\frac{\pi}{2}[$ and $\arctan(3)\in[0,\frac{\pi}{2}[$

$=\frac{-\pi}{4}+\pi=\frac{3\pi}{4}$

## Some more neat stuff

first of all: $\arcsin(x)+\arccos(x)=\frac{\pi}{2}$

the proof is as follows:

$$\begin{split}\sin(\arcsin(x)+\arccos(x)) \\= \sin(\arcsin(x))\cos(\arccos(x))+\sin(\arccos(x))\cos(\arcsin(x))\\=x\cdot x+\sqrt{1-x^{2}}\sqrt{1-x^{2}}\\=x^{2}-x^{2}+1\\=1\\\\\implies \arcsin(x)+\arccos(x)= \frac{\pi}{2}\end{split}$$

the last part is because we're only considering the interval $[0: \frac{\pi}{2}]$.

### Example

Find $AB\subseteq\mathbb{R}$ so that $f:A\to B$ defined using
$f(x)= 2\sin(\frac{\pi}{3}-x)+2\sin(x)$ would be bijective.

$$
\begin{equation}
\begin{split}
2(\sin(\frac{\pi}{3}-x)+\sin(x))=2(2\sin(\frac{\pi}{6})\cos(\frac{\pi}{6}-x)))\\
=2\cos(\frac{\pi}{6}-x)
\end{split}
\end{equation}
$$

This is defined on $[-2:2]$.

To choose A:

$\frac{pi}{6}-x\in[0;\pi]\iff0\le \frac{\pi}{6}+x\le \pi\iff \frac{-5\pi}{6}\le x\le \frac{pi}{6}$
Which means A is $[\frac{-5\pi}{6};\frac{\pi}{6}]$

The reciprocal of f, $f^{-1}$, is going to also need defining.

we solve $2\cos(\frac{\pi}{6}-x)=y$ where $y\in[-2;2]$ and $x\in[\frac{-5\pi}{6}: \frac{\pi}{6}]$.

$\cos(\frac{\pi}{6}-x)=\frac{y}{2}$
$\frac{\pi}{6}-x=\arccos(\frac{y}{2})$
$\frac{\pi}{6}-\arccos(\frac{y}{2})=x$

which means $f^{-1}: [-2;2]\to[\frac{-5\pi}{6}; \frac{\pi}{6}], x\to \frac{\pi}{6}-\arccos(\frac{x}{2})$.

### Another example

$\arcsin(x- \frac{1}{2})+\arcsin(\sqrt{2}x)=- \frac{\pi}{4}$

$D_{Def}=[\frac{-1}{2}, \frac{1}{\sqrt{2}}]$

$$\begin{split}\alpha=\arcsin(x- \frac{1}{2})\in[- \frac{\pi}{2}; \frac{\pi}{2}]\\ \beta=\arcsin(\sqrt{2}x)\in[-\pi;\pi]\\\text{results re theoretically possible.}\\\\ \alpha+\beta=\frac{-\pi}{4}\implies \sin(\alpha+\beta)=\sin(\frac{-\pi}{4})\\ \iff \text{after some steps you don't want to read and I don't want to write}\\\text{we get something that has square roots, monomials, and nothing simple looking.}\end{split}$$

So, we'll do this instead:

$$
\begin{split}
\alpha+\beta=- \frac{\pi}{4}\iff \alpha= \frac{-\pi}{4}-\beta\\\implies 
\sin(\alpha)=\sin(- \frac{\pi}{4}-\beta)\\
\iff \sin(x)=-[\sin(\frac{\pi}{4})\cos(\beta)+\sin(\beta)\cos(\beta)]\\
\iff (x-1)=[\frac{\sqrt{2}}{2}\sqrt{1-2x^{2}}+\sqrt{2x}\frac{\sqrt{2}}{2}]\\
\iff (x- \frac{1}{2})=- \frac{\sqrt{2}}{2}\sqrt{1-2x^{2}}-x\\
\iff 2x- \frac{1}{2}=- \frac{\sqrt{2}}{2}\sqrt{1-2x^{2}}\\
\iff (\frac{1}{2}-2x)^{2}=\frac{1}{2}(1-x^{2})\\
\iff \frac{1}{4}-4x^{2}=\frac{1}{2}-x^{2}\\
\iff 5x^{2}-2x- \frac{1}{4}=0\\
\iff (5x+ \frac{1}{2})(x- \frac{1}{2})=0\\
\iff x=- \frac{1}{10}
\end{split}
$$

(only -1/10 because $x\in[- \frac{1}{2}; \frac{1}{4}]$ due to it being in the definition (and positivity here) domains)

Next we need to test it of it works, which I'll leave as an exercise for the reader.

### Last example

$2\arctan(x)+\arctan(\sqrt{3}x)= \frac{-5\pi}{6}$

Ddef = R.

$\arctan(x)\in] \frac{-\pi}{2}; \frac{\pi}{2}[$

this means:

$$
\begin{split}
2\alpha+\beta\in ]\frac{-3\pi}{2};\frac{3\pi}{2}[\\
2\alpha-\beta= \frac{-5\pi}{6}\\
\implies\tan(2\alpha)=\tan(\frac{-5\pi}{6}-\beta)\\
\iff \frac{2\tan(\alpha)}{1-\tan^{2}(\alpha)}= \frac{\tan(\frac{-5\pi}{6})-\tan(\beta)}{1+\tan(\frac{-5\pi}{6})\tan(\beta)}\\
\iff \frac{2x}{1-x^{2}}= \frac{\frac{\sqrt{3}}{3}-\sqrt{3}x}{1+x}\\
\iff 2x= (\frac{\sqrt{3}}{3}-\sqrt{3}x)(1-x)\\
\iff\sqrt{3}x^{2}-x(\sqrt{3}+ \frac{\sqrt{3}}{3}+2)+ \frac{\sqrt{3}}{3}=0\\
\iff x_{1}\approx23, x_{2}\approx 0.14
\end{split}
$$

If we test these 2 values, we have the sum of both arctangents being positive, which is not possible given we're looking for a negative value.

Now we need to test if $x=\pm1$, because we've excluded it previously because tangent, but it's theoretically possible.

If we solve it, with -1 it's possible, meaning S={-1}.

[[7. Solving triangles|Previous]]
